Test/Eval.lean
@@ -2,10 +2,7 @@ import Nunchaku
 import Test.Eval.Sound
 import Test.Eval.Perf
 
--- TODO: handle False.rec
--- TODO: handle exists being used to build a dependent and
 -- TODO: handle casts
 
-
--- TODO: Figure out where Sum.rec is coming from
+-- TODO: This will be handle-able through casesOn handling
 #eval_nunchaku_sound_decl Sum.map_inl
